theories/Util/Wf_Uint63/Proofs.v
@@ -1,4 +1,4 @@
-From Coq Require Import Bool Uint63 ZArith Wellfounded Wf_Z Wf_nat Lia Setoid Morphisms.
+From Coq Require Import Zify ZifyUint63 Bool Uint63 ZArith Wellfounded Wf_Z Wf_nat Lia Setoid Morphisms.
 From NeuralNetInterp.Util Require Import Monad Notations Arith.Classes Arith.Instances Default.
 From NeuralNetInterp.Util.Tactics Require Import BreakMatch DestructHead UniquePose.
 From NeuralNetInterp.Util Require Import Wf_Uint63.
@@ -26,6 +26,214 @@ Module Reduction.
     cbn [Fix_F Acc_inv]; specialize (fun x y => IH _ (wf x y)).
     break_innermost_match; eauto.
   Qed.
+
+
+  Lemma map_reduce_no_init_spec {A reduce start0 stop step0 f} (P : int -> A -> Prop)
+    (step : int := if (step0 =? 0) then 1 else step0)
+    (start : int := start0 + step)
+    (Hinit : P start (f start0))
+    (Hstep : forall i v, P i v -> ((i + step) <? stop) = true -> P (i + step) (reduce v (f i)))
+    : P (start + step * (if start <? stop then (stop - start - 1) // step else 0))
+        (@map_reduce_no_init A reduce start0 stop step0 f).
+  Proof.
+    cbv [map_reduce_no_init start].
+    eapply for_loop_lt_invariant_gen
+      with (P:=fun i v
+               => P i v
+                  /\ ((i - start) mod step) = 0
+                  /\ (start <=? i) = true
+                  /\ ((start <? stop) = true -> i = start \/ ((i - step) <? stop) = true)
+                  /\ ((start <? stop) = false -> i = start)).
+    all: cbv [run_body Monad.bind LoopBody_Monad bind LoopNotation.get LoopNotation.set LoopNotation.update Classes.modulo Classes.sub Classes.add Classes.ltb int_has_modulo int_has_sub int_has_ltb int_has_leb Classes.leb int_has_add Classes.eqb int_has_eqb Classes.zero Classes.one int_has_zero int_has_one int_has_int_div Classes.int_div Classes.mul int_has_mul] in *.
+    { repeat apply conj; try assumption; subst step start; break_innermost_match.
+      all: lazymatch goal with
+           | [ |- ((?x mod ?y) = 0)%uint63 ]
+             => first [ replace x with y by lia | replace x with 0%uint63 by lia ];
+                assert (y / y = 1 /\ 0 / y = 0)%uint63; nia
+           | _ => try lia
+           end. }
+    3: { subst step start; break_innermost_match; intros; destruct_head'_and.
+         all: repeat match goal with H : _ |- _ => specialize (H eq_refl) end.
+         all: destruct_head'_or; subst.
+         all: try match goal with
+                | [ H : ?P ?x ?v |- ?P ?y ?v ] => replace y with x by lia
+                end.
+         all: try assumption.
+         clear H4.
+         assert (i = stop) by lia; subst.
+         (*
+         3: {
+         assert (start = (start + step0) - step0)%uint63 by lia.
+         generalize dependent (start + step0)%uint63; intro start'; intros; subst.
+         assert (i = start + (i - start))%uint63 by lia.
+         generalize dependent (i - start)%uint63; intro i'; intros; subst.
+         assert (stop = start + (stop - start))%uint63 by lia.
+         generalize dependent (stop - start)%uint63; intro len; intros; subst.
+         match goal with
+         | [ H : (?x mod ?y = 0)%uint63 |- _ ]
+           => let H' := fresh in
+              is_var x;
+              assert (y <> 0%uint63) by lia;
+              assert (x = y * (x / y))%uint63 by (clear -H H'; nia);
+              clear H;
+              generalize dependent (x / y)%uint63;
+              let x' := fresh in
+              rename x into x';
+              intro x; intros; subst
+         end.
+         assert (len = (len - 1) + 1)%uint63 by lia.
+         generalize dependent (len - 1)%uint63; intro len'; intros; subst.
+         assert ((step0 <=? step0 * i')%uint63 = true) by lia.
+         assert (len' = step0 * (len' / step0) + (len' mod step0))%uint63 by (clear; nia).
+         generalize dependent (len' / step0)%uint63; intro len; intros; subst.
+         assert ((0 <=? len' mod step0) = true)%uint63 by (clear; nia).
+         let H := lazymatch goal with H : step0 <> 0%uint63 |- _ => H end in
+         assert ((len' mod step0 <? step0) = true)%uint63 by (clear -H; nia).
+         generalize dependent (len' mod step0)%uint63; intro lenmod; intros; subst.
+         assert ((step0 * i' - step0 <? step0 * len + lenmod + 1) = true)%uint63 by lia.
+         match goal with
+                | [ H : ?P ?x ?v |- ?P ?y ?v ] => replace y with x by nia
+                end.
+         assert (step0
+         nia.
+         zify.
+         assert (
+         assert (
+         match goal with
+                | [ H : ?P ?x ?v |- ?P ?y ?v ] => replace y with x by nia
+                end.
+         assert (
+         nia.
+
+         Ltac zify_convert_to_euclidean_division_equations_flag ::= constr:(false).
+         zify.
+         rewrite Z.div_1_r.
+         rewrite Z.mul_1_l.
+         rewrite !Z.mod_mod by lia.
+
+         Ltac zify_convert_to_euclidean_division_equations_flag ::= constr:(true).
+         zify.
+         nia.
+         lia.
+
+         Z.to_euclidean_division_equations_
+         zify.
+
+         zify.
+         2: lia.
+         zify.
+      lia.
+      lia.
+      lia.
+      lia.
+      { clear.
+        subst step; break_innermost_match.
+        nia.
+        transitivity (step0 mod step0)%uint63; [ f_equal; lia | ].
+        assert (step0 / step0 = 1)%uint63; nia. }
+      subst step.
+
+    }
+
+      {
+      zify.
+      clear H3 H2.
+      clear H1.
+      specialize (H0 ltac:(lia)).
+      specialize (H ltac:(lia)).
+      generalize dependent (to_Z step0); clear step0; intros.
+
+      nia.
+
+      nia.
+      zify; lia.
+      zify.
+      nia.
+      zify. nia.
+      zify; Z.to_euclidean_division_equations; try nia.
+      break_innermost_match_hyps; subst; zify; try lia.
+      generalize dependent (to_Z step0); clear step0; intro step0; intros.
+      generalize dependent (to_Z step); clear step; intro step; intros.
+      generalize dependent (to_Z start); clear start; intro start; intros.
+      subst.
+      repeat match goal with H : _ |- _ => specialize (H ltac:(lia)) end.
+      assert (step0 <> 0)%Z by lia.
+      clear Heqb H3 H2.
+      clear H1.
+      clear H7 H6.
+      clear H11 H12.
+      subst.
+      clear H8.
+      clear H13.
+      assert (r1 = start + step0 - 9223372036854775808 * q1)%Z by lia.
+      clear H9.
+      subst.
+      assert ((step0 * (1 - q) - 9223372036854775808 * (q1 + q0) - ( r)%Z) = 0%Z)%Z by nia.
+      clear H4.
+      assert (0 <= q1 <= 1)%Z by nia.
+      assert (0 <= q0 + q1 <= 1)%Z by nia.
+      assert (-1 <= q0 <= 0)%Z by nia.
+      assert (0 <= q <= 1)%Z by nia.
+      assert (0 = q \/ 1 = q)%Z by lia.
+      destruct_head'_or; subst; lia.
+      assert (q0 + q1 = 0%Z) by nia.
+      assert (q0 = 0) by nia.
+      assert (q1 = 0) by nia.
+      nia.
+      subst.
+      clear H3 H2 H1.
+      clear Heqb cstr.
+      lia.
+      assert (r
+
+      zify.
+      zify.
+
+      Set Printing All.
+      zify.
+      assert (step0 = 0%Z).
+      Set Printing All.
+      zify.
+      Print Ltac Zify.zify.
+
+      { clear H13.
+        repeat match goal with H : _ |- _ => clear H; assert_succeeds (zify; [ | ]) end.
+        exfalso.
+        repeat match goal with H : _ |- _ => clear H; assert_succeeds (zify; [ | ]) end.
+        generalize dependent (@eqb int int_has_eqb); intro f; intros.
+        rename step0 into x.
+        assert
+        revert x f cstr4.
+  zify.
+  lia.
+
+
+        zify.
+        assert (step0 = 0%uint63).
+        Set Printing All.
+        zify.
+        zify.
+        zify.
+        zify.
+        zify.
+        Zify.zify_op.
+        Zify.zify_op.
+      Print Ltac zify.
+      zify.
+      zify.
+      zify.
+      zify.
+      zify.
+      zify.
+      zify.
+    Set Printing All.
+
+    eassumption.
+    Print for_loop_lt.
+    revert dependent start.
+          *)
+  Abort.
+
 
   Lemma argmax_gen_spec {A} {ltbA : has_ltb A} {start stop step f i v}
     (Hstep : step <> 0)
